Cleanup on aisle five.

isabelle/Countermodel.thy
@@ -1,212 +1,22 @@
 theory Countermodel
-  imports Hintikka
+  imports Hintikka Usemantics ProverLemmas
 begin
 
-section \<open>Alternative Semantics\<close>
+section \<open>Countermodels from Hintikka sets\<close>
 
-text \<open>We define an alternate semantics where the quantifiers refer to a specific set\<close>
-primrec usemantics where
-  \<open>usemantics u e f g (Pre i l) = g i (semantics_list e f l)\<close> |
-  \<open>usemantics u e f g (Imp p q) = (usemantics u e f g p \<longrightarrow> usemantics u e f g q)\<close> |
-  \<open>usemantics u e f g (Dis p q) = (usemantics u e f g p \<or> usemantics u e f g q)\<close> |
-  \<open>usemantics u e f g (Con p q) = (usemantics u e f g p \<and> usemantics u e f g q)\<close> |
-  \<open>usemantics u e f g (Exi p) = (\<exists>x \<in> u. usemantics u (SeCaV.shift e 0 x) f g p)\<close> |
-  \<open>usemantics u e f g (Uni p) = (\<forall>x \<in> u. usemantics u (SeCaV.shift e 0 x) f g p)\<close> |
-  \<open>usemantics u e f g (Neg p) = (\<not> usemantics u e f g p)\<close>
+text \<open>A predicate is satisfied in a set of formulas S if its negation is also in S\<close>
+abbreviation (input) \<open>sat S n ts \<equiv> Neg (Pre n ts) \<in> S\<close>
 
-text \<open>An environment is only defined if the variables are actually in the quantifier set u\<close>
-definition is_env :: \<open>'a set \<Rightarrow> (nat \<Rightarrow> 'a) \<Rightarrow> bool\<close> where
-  \<open>is_env u e \<equiv> \<forall>n. e n \<in> u\<close>
+text \<open>Alternate interpretation for environments: if a variable is not present, we interpret it as some existing term\<close>
+abbreviation \<open>E S n \<equiv> if Var n \<in> terms S then Var n else SOME t. t \<in> terms S\<close>
 
-definition is_fdenot :: \<open>'a set \<Rightarrow> (nat \<Rightarrow> 'a list \<Rightarrow> 'a) \<Rightarrow> bool\<close> where
-  \<open>is_fdenot u f \<equiv> \<forall>i l. list_all (\<lambda>x. x \<in> u) l \<longrightarrow> f i l \<in> u\<close>
+abbreviation \<open>F S i l \<equiv> if Fun i l \<in> terms S then Fun i l else SOME t. t \<in> terms S\<close>
 
-text \<open>A formula only needs to be valid for the "real" environments\<close>
-(* TODO: change this *)
-definition uvalid :: \<open>'a set \<Rightarrow> fm \<Rightarrow> bool\<close> where
-  \<open>uvalid u p \<equiv> \<forall>e f g. is_env u e \<longrightarrow> is_fdenot u f \<longrightarrow> usemantics u e f g p\<close>
-
-text \<open>If we choose to quantify over the universal set, we obtain the usual semantics\<close>
-lemma usemantics_UNIV: \<open>usemantics UNIV e f g p \<longleftrightarrow> semantics e f g p\<close>
-  by (induct p arbitrary: e) auto
-
-text \<open>If we choose the universal set, any environment is defined\<close>
-lemma is_env_UNIV: \<open>is_env UNIV e\<close>
-  unfolding is_env_def by blast
-
-text \<open>If a formula is valid for any quantifier set, it is valid for the universal set in particular,
-and we thus obtain that it is also valid in the usual semantics\<close>
-lemma uvalid_semantics:
-  fixes e :: \<open>nat \<Rightarrow> 'a\<close>
-  assumes \<open>\<forall>(u :: 'a set) e f g. usemantics u e f g p\<close>
-  shows \<open>semantics e f g p\<close>
-  using assms is_env_UNIV usemantics_UNIV by blast
-
-lemma uupd_lemma [iff]: \<open>n \<notin> params p \<Longrightarrow> usemantics u e (f(n := z)) g p \<longleftrightarrow> usemantics u e f g p\<close>
-  by (induct p arbitrary: e) simp_all
-
-text \<open>The semantics of substituting variable i by term t in formula a are well-defined\<close>
-lemma usubst_lemma [iff]:
-  \<open>usemantics u e f g (subst a t i) \<longleftrightarrow> usemantics u (SeCaV.shift e i (semantics_term e f t)) f g a\<close>
-  by (induct a arbitrary: e i t) simp_all
-
-subsection \<open>Soundness of SeCaV\<close>
-
-lemma usemantics_term [simp]:
-  assumes \<open>is_env u e\<close> \<open>is_fdenot u f\<close>
-  shows \<open>semantics_term e f t \<in> u\<close> \<open>list_all (\<lambda>x. x \<in> u) (semantics_list e f l)\<close>
-  using assms by (induct t and l rule: semantics_term.induct semantics_list.induct)
-    (simp_all add: is_env_def is_fdenot_def)
-
-lemma is_env_shift [simp]: \<open>is_env u e \<Longrightarrow> x \<in> u \<Longrightarrow> is_env u (SeCaV.shift e v x)\<close>
-  unfolding is_env_def SeCaV.shift_def by simp                  
-
-lemma is_fdenot_shift [simp]: \<open>is_fdenot u f \<Longrightarrow> x \<in> u \<Longrightarrow> is_fdenot u (f(i := \<lambda>_. x))\<close>
-  unfolding is_fdenot_def SeCaV.shift_def by simp
-
-theorem sound_usemantics:
-  assumes \<open>\<tturnstile> z\<close> \<open>is_env u e\<close> \<open>is_fdenot u f\<close>
-  shows \<open>\<exists>p \<in> set z. usemantics u e f g p\<close>
-  using assms
-proof (induct arbitrary: f rule: sequent_calculus.induct)
-  case (10 i p z)
-  then show ?case
-  proof (cases \<open>\<forall>x \<in> u. usemantics u e (f(i := \<lambda>_. x)) g (sub 0 (Fun i []) p)\<close>)
-    case False
-    moreover have \<open>\<forall>x \<in> u. \<exists>p \<in> set (sub 0 (Fun i []) p # z). usemantics u e (f(i := \<lambda>_. x)) g p\<close>
-      using 10 is_fdenot_shift by metis
-    ultimately have \<open>\<exists>x \<in> u. \<exists>p \<in> set z. usemantics u e (f(i := \<lambda>_. x)) g p\<close>
-      by fastforce
-    moreover have \<open>list_all (\<lambda>p. i \<notin> params p) z\<close>
-      using 10 by simp
-    ultimately show ?thesis
-      using 10 Ball_set insert_iff list.set(2) uupd_lemma by metis
-  qed simp
-next
-  case (11 i p z)
-  then show ?case
-  proof (cases \<open>\<forall>x \<in> u. usemantics u e (f(i := \<lambda>_. x)) g (Neg (sub 0 (Fun i []) p))\<close>)
-    case False
-    moreover have
-      \<open>\<forall>x \<in> u. \<exists>p \<in> set (Neg (sub 0 (Fun i []) p) # z). usemantics u e (f(i := \<lambda>_. x)) g p\<close>
-      using 11 is_fdenot_shift by metis
-    ultimately have \<open>\<exists>x \<in> u. \<exists>p \<in> set z. usemantics u e (f(i := \<lambda>_. x)) g p\<close>
-      by fastforce
-    moreover have \<open>list_all (\<lambda>p. i \<notin> params p) z\<close>
-      using 11 by simp
-    ultimately show ?thesis
-      using 11 Ball_set insert_iff list.set(2) uupd_lemma by metis
-  qed simp
-qed fastforce+
-
-section \<open>Machinery\<close>
-
-text \<open>If t is a term in some argument list ts, t is also in the list of subterms of a function
-applied to those arguments\<close>
-lemma subtermTm_Fun: \<open>t \<in> set ts \<longrightarrow> t \<in> set (subtermTm (Fun i ts))\<close>
-proof (induction ts)
-  case Nil
-  then show ?case by simp
-next
-  case (Cons t' ts')
-  then show ?case
-  proof (safe)
-    assume \<open>t \<in> set (t' # ts')\<close> \<open>t \<notin> set ts'\<close>
-    from this have \<open>t = t'\<close> by simp
-    moreover have \<open>t' \<in> set (subtermTm (Fun i (t' # ts')))\<close>
-    proof (simp)
-      have \<open>t' \<in> set (subtermTm t')\<close>
-        by (cases t') simp_all
-      then show \<open>t' = Fun i (t' # ts') \<or> t' \<in> set (subtermTm t') \<or> (\<exists>x\<in>set ts'. t' \<in> set (subtermTm x))\<close>
-        by simp
-    qed
-    ultimately show \<open>t \<in> set (subtermTm (Fun i (t' # ts')))\<close> by simp
-  next
-    assume \<open>t \<in> set (t' # ts')\<close> \<open>t \<in> set (subtermTm (Fun i ts'))\<close>
-    then show \<open>t \<in> set (subtermTm (Fun i (t' # ts')))\<close>
-    proof (simp)
-      assume *: \<open>t = t' \<or> t \<in> set ts'\<close>
-      assume \<open>t = Fun i ts' \<or> (\<exists>x\<in>set ts'. t \<in> set (subtermTm x))\<close>
-      then show \<open>t = Fun i (t' # ts') \<or> t \<in> set (subtermTm t') \<or> (\<exists>x\<in>set ts'. t \<in> set (subtermTm x))\<close>
-      proof (cases \<open>\<exists>x\<in>set ts'. t \<in> set (subtermTm x)\<close>)
-        case True
-        then show ?thesis by simp
-      next
-        case False
-        then show ?thesis
-        proof (cases \<open>t = t'\<close>)
-          case True
-          then show ?thesis
-          proof (simp)
-            have \<open>t' \<in> set (subtermTm t')\<close>
-              by (cases t') simp_all
-            then show \<open>t' = Fun i (t' # ts') \<or> t' \<in> set (subtermTm t') \<or> (\<exists>x\<in>set ts'. t' \<in> set (subtermTm x))\<close>
-              by simp
-          qed
-        next
-          case False
-          then show ?thesis
-          proof -
-            have \<open>t \<in> set ts'\<close>
-              using * False by simp
-            moreover have \<open>t \<in> set (subtermTm t)\<close>
-              by (cases t) simp_all
-            ultimately have \<open>\<exists>x \<in> set ts'. t \<in> set (subtermTm x)\<close>
-              by blast
-            then show \<open>t = Fun i (t' # ts') \<or> t \<in> set (subtermTm t') \<or> (\<exists>x\<in>set ts'. t \<in> set (subtermTm x))\<close>
-              by simp
-          qed
-        qed
-      qed
-    qed
-  qed
-qed
-
-lemma subtermTm_refl [simp]: \<open>t \<in> set (subtermTm t)\<close>
-  by (induct t) simp_all
-
-lemma subterm_Pre_refl: \<open>set ts \<subseteq> set (subtermFm (Pre n ts))\<close>
-  by (induct ts) auto
-
-lemma subterm_Fun_refl: \<open>set ts \<subseteq> set (subtermTm (Fun n ts))\<close>
-  by (induct ts) auto
+lemma terms_ne [simp]: \<open>terms S \<noteq> {}\<close>
+  unfolding terms_def by simp
 
 lemma terms_cases: \<open>t \<in> terms S \<Longrightarrow> t = Fun 0 [] \<or> (\<exists>p \<in> S. t \<in> set (subtermFm p))\<close>
   unfolding terms_def by (simp split: if_splits)
-
-primrec preds :: \<open>fm \<Rightarrow> fm set\<close> where
-  \<open>preds (Pre n ts) = {Pre n ts}\<close>
-| \<open>preds (Imp f1 f2) = preds f1 \<union> preds f2\<close>
-| \<open>preds (Dis f1 f2) = preds f1 \<union> preds f2\<close>
-| \<open>preds (Con f1 f2) = preds f1 \<union> preds f2\<close>
-| \<open>preds (Exi f) = preds f\<close>
-| \<open>preds (Uni f) = preds f\<close>
-| \<open>preds (Neg f) = preds f\<close>
-
-lemma subtermFm_preds: \<open>t \<in> set (subtermFm p) \<longleftrightarrow> (\<exists>pre \<in> preds p. t \<in> set (subtermFm pre))\<close>
-  by (induct p) auto
-
-lemma preds_shape: \<open>pre \<in> preds p \<Longrightarrow> \<exists>n ts. pre = Pre n ts\<close>
-  by (induct p) auto
-
-lemma subtermTm_le: \<open>t \<in> set (subtermTm s) \<Longrightarrow> set (subtermTm t) \<subseteq> set (subtermTm s)\<close>
-  by (induct s) auto
-
-lemma fun_arguments_subterm:
-  assumes \<open>Fun n ts \<in> set (subtermFm p)\<close>
-  shows \<open>set ts \<subseteq> set (subtermFm p)\<close>
-proof -
-  obtain pre where pre: \<open>pre \<in> preds p\<close> \<open>Fun n ts \<in> set (subtermFm pre)\<close>
-    using assms subtermFm_preds by blast
-  then obtain n' ts' where \<open>pre = Pre n' ts'\<close>
-    using preds_shape by blast
-  then have \<open>set ts \<subseteq> set (subtermFm pre)\<close>
-    using subtermTm_le pre by force
-  then have \<open>set ts \<subseteq> set (subtermFm p)\<close>
-    using pre subtermFm_preds by blast
-  then show ?thesis
-    by blast
-qed
 
 lemma terms_downwards_closed: \<open>t \<in> terms S \<Longrightarrow> set (subtermTm t) \<subseteq> terms S\<close>
 proof (induct t)
@@ -243,19 +53,6 @@ next
     by simp
 qed
 
-section \<open>Countermodels from Hintikka sets\<close>
-
-text \<open>A predicate is satisfied in a set of formulas S if its negation is also in S\<close>
-abbreviation (input) \<open>sat S n ts \<equiv> Neg (Pre n ts) \<in> S\<close>
-
-text \<open>Alternate interpretation for environments: if a variable is not present, we interpret it as some existing term\<close>
-abbreviation \<open>E S n \<equiv> if Var n \<in> terms S then Var n else SOME t. t \<in> terms S\<close>
-
-abbreviation \<open>F S i l \<equiv> if Fun i l \<in> terms S then Fun i l else SOME t. t \<in> terms S\<close>
-
-lemma terms_ne [simp]: \<open>terms S \<noteq> {}\<close>
-  unfolding terms_def by simp
-
 text \<open>If terms are actually in a set of formulas, interpreting the environment over these formulas
 allows for a Herbrand interpretation\<close>
 lemma usemantics_E:
@@ -265,29 +62,12 @@ lemma usemantics_E:
 proof (induct t and ts arbitrary: ts rule: semantics_term.induct semantics_list.induct)
   case (Fun i ts')
   moreover have \<open>\<forall>t' \<in> set ts'. t' \<in> set (subtermTm (Fun i ts'))\<close>
-    using subtermTm_Fun by blast
+    using subterm_Fun_refl by blast
   ultimately have \<open>list_all (\<lambda>t. t \<in> terms S) ts'\<close>
     using terms_downwards_closed unfolding list_all_def by (metis (no_types, lifting) subsetD)
   then show ?case
     using Fun by simp
-next
-  case (Var x)
-  then show ?case
-    by fastforce
-next
-  case Nil_tm
-  then show ?case
-    by simp
-next
-  case (Cons_tm x1 x2)
-  then show ?case
-    by simp
-qed
-
-text \<open>Substituting a variable by a term does not change the depth of a formula
-(only the term size changes)\<close>
-lemma size_sub [simp]: \<open>size (sub i t p) = size p\<close>
-  by (induct p arbitrary: i t) auto
+qed simp_all
 
 text \<open>As long as some formulas exist, our alternate interpretation of environments is defined\<close>
 lemma is_env_E: \<open>is_env (terms S) (E S)\<close>
@@ -475,6 +255,5 @@ next
     qed
   qed
 qed
-
 
 end
