isabelle/Completeness.thy
@@ -1,100 +1,94 @@
 theory Completeness
-  imports Countermodel "Sequent_Calculus_Verifier" "HOL-Library.BNF_Corec"
+  imports Countermodel EPathHintikka "Sequent_Calculus_Verifier" "HOL-Library.BNF_Corec"
 begin
 
 section \<open>Completeness of the prover\<close>
 
 text \<open>We start out by specializing the abstract completeness theorem to our prover\<close>
 theorem epath_prover_completeness:
-  fixes A :: \<open>tm list\<close> and p :: fm
-  defines \<open>t \<equiv> secavProver (A, [p])\<close>
+  fixes A :: \<open>tm list\<close> and ps :: \<open>fm list\<close>
+  defines \<open>t \<equiv> secavProver (A, ps)\<close>
   shows
-  "(fst (root t) = (A, [p]) \<and> wf t \<and> tfinite t) \<or>
-   (\<exists> steps. fst (shd steps) = (A, [p]) \<and> epath steps \<and> Saturated steps)" (is "?A \<or> ?B")
+    \<open>(fst (root t) = (A, ps) \<and> wf t \<and> tfinite t) \<or>
+   (\<exists> steps. fst (shd steps) = (A, ps) \<and> epath steps \<and> Saturated steps)\<close> (is \<open>?A \<or> ?B\<close>)
 proof -
-  { assume "\<not> ?A"
-    with assms have "\<not> tfinite (mkTree rules (A, [p]))"
+  { assume \<open>\<not> ?A\<close>
+    with assms have \<open>\<not> tfinite (mkTree rules (A, ps))\<close>
       unfolding secavProver_def using wf_mkTree fair_rules by simp
-    then obtain steps where "ipath (mkTree rules (A, [p])) steps" using Konig by blast
-    with assms have "fst (shd steps) = (A, [p]) \<and> epath steps \<and> Saturated steps"
+    then obtain steps where \<open>ipath (mkTree rules (A, ps)) steps\<close> using Konig by blast
+    with assms have \<open>fst (shd steps) = (A, ps) \<and> epath steps \<and> Saturated steps\<close>
       by (metis UNIV_I fair_rules ipath.cases ipath_mkTree_Saturated mkTree.simps(1) prod.sel(1)
           wf_ipath_epath wf_mkTree)
-    hence ?B by blast
+    then have ?B by blast
   }
-  thus ?thesis by blast
+  then show ?thesis by blast
 qed
 
 section \<open>Generating countermodels from saturated escape paths\<close>
 
+abbreviation \<open>uvalid ps \<equiv> \<forall>u (e :: nat \<Rightarrow> tm) f g. is_env u e \<longrightarrow> is_fdenot u f \<longrightarrow>
+      (\<exists>p \<in> set ps. usemantics u e f g p)\<close>
+
 text \<open>We need some lemmas to prove our main theorem\<close>
 lemma epath_countermodel:
-  assumes \<open>\<exists> steps. fst (shd steps) = (A, [p]) \<and> epath steps \<and> Saturated steps\<close>
-  shows \<open>\<exists>u (e :: nat \<Rightarrow> tm) f g . \<not> usemantics u e f g p \<and> is_env u e \<and> is_fdenot u f\<close>
-proof (rule ccontr)
-  assume \<open>\<nexists>u (e :: nat \<Rightarrow> tm) f g. \<not> usemantics u e f g p \<and> is_env u e \<and> is_fdenot u f\<close>
-  then have \<open>\<forall>u (e :: nat \<Rightarrow> tm) f g. is_env u e \<longrightarrow> is_fdenot u f \<longrightarrow> usemantics u e f g p\<close>
+  assumes \<open>fst (shd steps) = (A, ps)\<close> \<open>epath steps\<close> \<open>Saturated steps\<close>
+  shows \<open>\<not> uvalid ps\<close>
+proof
+  assume \<open>uvalid ps\<close>
+  moreover obtain steps where steps: \<open>fst (shd steps) = (A, ps) \<and> epath steps \<and> Saturated steps\<close>
+    using assms by blast
+  then have \<open>Hintikka (tree_fms steps)\<close> (is \<open>Hintikka ?S\<close>)
+    using escape_path_Hintikka assms by simp
+  moreover have \<open>\<forall>p \<in> set ps. p \<in> tree_fms steps\<close>
+    using steps shd_sset by (metis Pair_inject prod.collapse pseq_def pseq_in_tree_fms)
+  then have \<open>\<exists>g. \<forall>p \<in> set ps. \<not> usemantics (terms ?S) (E ?S) (F ?S) g p\<close>
+    using calculation(2) hintikka_counter_model steps by blast
+  moreover have \<open>is_env (terms ?S) (E ?S)\<close> \<open>is_fdenot (terms ?S) (F ?S)\<close>
+    using is_env_E is_fdenot_F by blast+
+  ultimately show False
     by blast
-  then show False
-  proof -
-    assume \<open>\<forall>u (e :: nat \<Rightarrow> tm) f g. is_env u e \<longrightarrow> is_fdenot u f \<longrightarrow> usemantics u e f g p\<close>
-    moreover obtain steps
-      where steps: \<open>fst (shd steps) = (A, [p]) \<and> epath steps \<and> Saturated steps\<close>
-      using assms by blast
-    then have \<open>Hintikka (tree_fms steps)\<close> (is \<open>Hintikka ?S\<close>)
-      using escape_path_Hintikka assms by simp
-    moreover have \<open>p \<in> tree_fms steps\<close>
-      using steps shd_sset
-      by (metis Pair_inject list.set_intros(1) prod.collapse pseq_def pseq_in_tree_fms)
-    then have \<open>\<exists>g. \<not> usemantics (terms ?S) (E ?S) (F ?S) g p\<close>
-      using calculation(2) hintikka_counter_model steps by blast
-    moreover have \<open>is_env (terms ?S) (E ?S)\<close> \<open>is_fdenot (terms ?S) (F ?S)\<close>
-      using is_env_E is_fdenot_F by blast+
-    ultimately show False
-      by blast
-  qed
 qed
 
 lemma epath_lem:
-  assumes \<open>\<nexists> steps. fst (shd steps) = (A, [p]) \<and> epath steps \<and> Saturated steps\<close>
-  defines \<open>t \<equiv> secavProver (A, [p])\<close>
-  shows \<open>fst (root t) = (A, [p]) \<and> wf t \<and> tfinite t\<close>
+  assumes \<open>\<nexists>steps. fst (shd steps) = (A, ps) \<and> epath steps \<and> Saturated steps\<close>
+  defines \<open>t \<equiv> secavProver (A, ps)\<close>
+  shows \<open>fst (root t) = (A, ps) \<and> wf t \<and> tfinite t\<close>
   using assms epath_prover_completeness t_def by blast
 
 lemma epath_contr:
-  assumes \<open>\<forall>(u :: tm set) e f g. is_env u e \<longrightarrow> is_fdenot u f \<longrightarrow> usemantics u e f g p\<close>
-  shows \<open>\<nexists> steps. fst (shd steps) = (A, [p]) \<and> epath steps \<and> Saturated steps\<close>
-proof (rule ccontr, safe)
-  fix steps
-  assume \<open>fst (shd steps) = (A, [p])\<close> \<open>epath steps\<close> \<open>Saturated steps\<close>
+  assumes \<open>\<forall>u (e :: nat \<Rightarrow> tm) f g. is_env u e \<longrightarrow> is_fdenot u f \<longrightarrow>
+      (\<exists>p \<in> set ps. usemantics u e f g p)\<close>
+  shows \<open>\<nexists>steps. fst (shd steps) = (A, ps) \<and> epath steps \<and> Saturated steps\<close>
+proof
+  assume \<open>\<exists>steps. fst (shd steps) = (A, ps) \<and> epath steps \<and> Saturated steps\<close>
   then obtain u f g and e :: \<open>nat \<Rightarrow> tm\<close> where
-    \<open>\<not> usemantics u e f g p\<close> \<open>is_env u e\<close> \<open>is_fdenot u f\<close>
+    \<open>\<forall>p \<in> set ps. \<not> usemantics u e f g p\<close> \<open>is_env u e\<close> \<open>is_fdenot u f\<close>
     using epath_countermodel by blast
   with assms show False
-    by simp
+    by blast
 qed
 
 text \<open>Finally, we arrive at the main theorem\<close>
-
-theorem completeness_usemantics:
+theorem prover_completeness_usemantics:
   fixes A :: \<open>tm list\<close>
-  assumes \<open>\<forall>(u :: tm set) e f g. is_env u e \<longrightarrow> is_fdenot u f \<longrightarrow> usemantics u e f g p\<close>
-  defines \<open>t \<equiv> secavProver (A, [p])\<close>
-  shows \<open>fst (root t) = (A, [p]) \<and> wf t \<and> tfinite t\<close>
-  by (simp add: assms epath_contr epath_lem epath_prover_completeness)
+  assumes \<open>uvalid ps\<close>
+  defines \<open>t \<equiv> secavProver (A, ps)\<close>
+  shows \<open>fst (root t) = (A, ps) \<and> wf t \<and> tfinite t\<close>
+  using assms by (simp add: epath_contr epath_lem epath_prover_completeness)
 
-corollary completeness_SeCaV:
+corollary prover_completeness_SeCaV:
   fixes A :: \<open>tm list\<close>
-  assumes \<open>\<tturnstile> [p]\<close>
-  defines \<open>t \<equiv> secavProver (A, [p])\<close>
-  shows \<open>fst (root t) = (A, [p]) \<and> wf t \<and> tfinite t\<close>
+  assumes \<open>\<tturnstile> ps\<close>
+  defines \<open>t \<equiv> secavProver (A, ps)\<close>
+  shows \<open>fst (root t) = (A, ps) \<and> wf t \<and> tfinite t\<close>
 proof -
-  have \<open>\<forall>(u :: tm set) e f g. is_env u e \<longrightarrow> is_fdenot u f \<longrightarrow> usemantics u e f g p\<close>
-    using assms sound_usemantics by fastforce
+  have \<open>uvalid ps\<close>
+    using assms sound_usemantics by blast
   then show ?thesis
-    using assms completeness_usemantics by blast
+    using assms prover_completeness_usemantics by blast
 qed
 
-corollary completeness_semantics:
+corollary prover_completeness_semantics:
   fixes A :: \<open>tm list\<close>
   assumes \<open>\<forall>(e :: nat \<Rightarrow> nat hterm) f g. semantics e f g p\<close>
   defines \<open>t \<equiv> secavProver (A, [p])\<close>
@@ -103,7 +97,7 @@ proof -
   have \<open>\<tturnstile> [p]\<close>
     using assms complete_sound(1) by blast
   then show ?thesis
-    using assms completeness_SeCaV by blast
+    using assms prover_completeness_SeCaV by blast
 qed
 
 end
