isabelle/Results.thy
@@ -1,0 +1,37 @@
+theory Results imports Soundness Completeness begin
+
+theorem prover_SeCaV:
+  fixes A :: \<open>tm list\<close> and ps :: \<open>fm list\<close>
+  defines \<open>t \<equiv> secavProver (A, ps)\<close>
+  shows \<open>tfinite t \<and> wf t \<longleftrightarrow> (\<tturnstile> ps)\<close>
+  using assms prover_soundness_SeCaV prover_completeness_SeCaV
+  unfolding secavProver_def by fastforce
+
+corollary
+  fixes p :: fm
+  defines \<open>t \<equiv> secavProver ([], [p])\<close>
+  shows \<open>tfinite t \<and> wf t \<longleftrightarrow> (\<tturnstile> [p])\<close>
+  using assms prover_SeCaV by blast
+
+theorem prover_usemantics:
+  fixes A :: \<open>tm list\<close> and ps :: \<open>fm list\<close>
+  defines \<open>t \<equiv> secavProver (A, ps)\<close>
+  shows \<open>tfinite t \<and> wf t \<longleftrightarrow> (uvalid ps)\<close>
+  using assms prover_soundness_usemantics prover_completeness_usemantics
+  unfolding secavProver_def by fastforce
+
+corollary
+  fixes p :: fm
+  defines \<open>t \<equiv> secavProver ([], [p])\<close>
+  shows \<open>tfinite t \<and> wf t \<longleftrightarrow> (\<forall>(u :: tm set) e f g.
+    is_env u e \<longrightarrow> is_fdenot u f \<longrightarrow> usemantics u e f g p)\<close>
+  using assms prover_usemantics by simp
+
+theorem prover_semantics:
+  fixes A :: \<open>tm list\<close> and p :: fm
+  defines \<open>t \<equiv> secavProver (A, [p])\<close>
+  shows \<open>tfinite t \<and> wf t \<longleftrightarrow> (\<forall>(e :: nat \<Rightarrow> nat hterm) f g. semantics e f g p)\<close>
+  using assms prover_soundness_semantics prover_completeness_semantics
+  unfolding secavProver_def by fastforce
+
+end
